prove cellio cancellation (draft)

cellio/CellioA.v
@@ -3,30 +3,31 @@ Require Import CellioHeader CtxHeader.
 
 Set Implicit Arguments.
 
-Section CellioRA.
-  Context `{!crisG Γ Σ α β τ _S _I}.
+Local Definition RA : ucmra :=
+  authUR (optionUR (exclR ZO)).
+Class cellioGpreS `{!crisG Γ Σ α β τ _S _I} := {
+  #[local] cellio_inG :: inG RA Γ;
+}.
+Class cellioGS `{!crisG Γ Σ α β τ _S _I} := {
+  #[local] cellioGS_cellioGpreS :: cellioGpreS;
+  cell_name : gname;
+}.
+Definition cellioΓ : HRA := #[RA].
+Global Instance subG_cellioG `{!crisG Γ Σ α β τ _S _I} :
+  subG cellioΓ Γ → cellioGpreS.
+Proof. solve_inG. Defined.
 
-  Local Definition RA : ucmra :=
-    authUR (optionUR (exclR ZO)).
-
-  Class cellioG `{!crisG Γ Σ α β τ _S _I} := {
-    cellio_inG :: inG RA Γ;
-  }.
-  Definition cellioΓ : HRA := #[RA].
-  Global Instance subG_cellioG : subG cellioΓ Γ → cellioG.
-  Proof. solve_inG. Defined.
-End CellioRA.  
-Hint Unfold subG_cellioG cellio_inG : GRA_index.
+Local Existing Instances cellioGS_cellioGpreS cellio_inG.
 
 Module CellioA. Section CellioA.
   Context `{!crisG Γ Σ α β τ _S _I}.
-  Context `{_CELLIO: !cellioG}.
+  Context `{_CELLIO: !cellioGS}.
 
   Definition auth (v : Z) : iProp Σ :=
-    own base_γ (●E v).
+    own cell_name (●E v).
 
   Definition cell (v : Z) : iProp Σ :=
-    own base_γ (◯E v).
+    own cell_name (◯E v).
 
   Lemma cell_auth_get v v':
     cell v -∗ auth v' -∗ ⌜v = v'⌝.
@@ -80,3 +81,13 @@ Module CellioA. Section CellioA.
   (* We can use ∅ because Cellio will be removed before cancellation *)
   Definition t := SMod.to_mod ∅ smod.
 End CellioA. End CellioA.
+
+Lemma cellio_alloc `{!crisG Γ Σ α β τ Hsub Hinv, !cellioGpreS} :
+  ⊢ o=> ∃ (_ : cellioGS), CellioA.init_cond ∗ CellioA.cell 0.
+Proof.
+  iMod (own_alloc (●E 0%Z ⋅ ◯E 0%Z)) as "[%γt T]".
+  { apply auth_both_valid_discrete; esplits; ss. }
+  pose (Build_cellioGS _ γt) as Hcell.
+  rewrite own_op; iExists Hcell. iDestruct "T" as "[T0 T1]"; iFrame.
+  done.
+Qed.
