cellio/CellioIAproof.v
@@ -7,7 +7,7 @@ Local Open Scope nat_scope.
 
 Module CellioIA. Section CellioIA.
   Import CellioA.
-  Context `{!crisG Γ Σ α β τ _S _I, _CELLIO: !cellioG}.
+  Context `{!crisG Γ Σ α β τ _S _I, _CELLIO: !cellioGS}.
 
   Definition Ist : ist_type Σ :=
     fun st_src st_tgt =>
